src/Term_system.v
@@ -23,7 +23,7 @@ Set Nested Proofs Allowed.
 Fixpoint ev_sys (t: AnnoTerm) p: EvSys Ev :=
   match t with
   | aasp (i, j) lr x => leaf (i, j) (asp_event i x p)
-  | aatt (i, j) lr (req_loc,rpy_loc) p' q x =>
+  | aatt (i, j) lr (req_loc,rpy_loc) p' q m x =>
     before (i, j)
       (leaf (i, S i) (req i req_loc p q (*(unanno x)*)))
       (before (S i, j)
